Rename functions for consistency

src/c/include/coq-vsu-certicoq-block/block.h
@@ -13,22 +13,22 @@ certicoq_block_t certicoq_block__init(int_or_ptr *dst, const certicoq_block_head
 certicoq_block_t certicoq_block__of_header(certicoq_block_header_t *header);
 certicoq_block_t certicoq_block__copy(int_or_ptr *dst, const certicoq_block_t src);
 
-certicoq_block_header_t *certicoq_block__get_header_ptr(const certicoq_block_t block);
-void certicoq_block__set_header(certicoq_block_t block, const certicoq_block_header_t *header);
+certicoq_block_header_t *certicoq_block__header_get_ptr(const certicoq_block_t block);
+void certicoq_block__header_set(certicoq_block_t block, const certicoq_block_header_t *header);
 
-size_t certicoq_block__get_size(const certicoq_block_header_t *header);
+size_t certicoq_block__size_get(const certicoq_block_header_t *header);
 
-size_t certicoq_block__get_field_count(const certicoq_block_header_t *header);
-void certicoq_block__set_field_count(certicoq_block_header_t *header, size_t size);
+size_t certicoq_block__field_count_get(const certicoq_block_header_t *header);
+void certicoq_block__field_count_set(certicoq_block_header_t *header, size_t size);
 
-certicoq_block_tag_t certicoq_block__get_tag(const certicoq_block_header_t *header);
-certicoq_block_header_t certicoq_block__set_tag(certicoq_block_header_t *header, certicoq_block_tag_t tag);
+certicoq_block_tag_t certicoq_block__tag_get(const certicoq_block_header_t *header);
+void certicoq_block__tag_set(certicoq_block_header_t *header, certicoq_block_tag_t tag);
 
-uint8_t certicoq_block__get_odata(const certicoq_block_header_t *header);
-void certicoq_block__set_odata(certicoq_block_header_t *header, uint8_t odata);
+uint8_t certicoq_block__odata_get(const certicoq_block_header_t *header);
+void certicoq_block__odata_set(certicoq_block_header_t *header, uint8_t odata);
 
-int_or_ptr *certicoq_block__get_field_ptr(certicoq_block_t block, size_t field);
-int_or_ptr certicoq_block__get_field(const certicoq_block_t block, size_t field);
-void certicoq_block__set_field(certicoq_block_t block, size_t field, int_or_ptr x);
+int_or_ptr *certicoq_block__field_get_ptr(certicoq_block_t block, size_t field);
+int_or_ptr certicoq_block__field_get(const certicoq_block_t block, size_t field);
+void certicoq_block__field_set(certicoq_block_t block, size_t field, int_or_ptr x);
 
 #endif /* COQ_CERTICOQ_BLOCK__BLOCK_H */
