src/c/include/coq-vsu-certicoq-block/src/block.c
@@ -6,7 +6,7 @@
 certicoq_block_t certicoq_block__init(int_or_ptr *dst, const certicoq_block_header_t *header)
 {
     certicoq_block_t ret = dst + 1;
-    certicoq_block__set_header(ret, header);
+    certicoq_block__header_set(ret, header);
     return ret;
 }
 
@@ -17,78 +17,78 @@ certicoq_block_t certicoq_block__of_header(certicoq_block_header_t *header)
 
 certicoq_block_t certicoq_block__copy(int_or_ptr *dst, const certicoq_block_t src)
 {
-    certicoq_block_header_t *hd = certicoq_block__get_header_ptr(src);
+    certicoq_block_header_t *hd = certicoq_block__header_get_ptr(src);
     certicoq_block_t ret = certicoq_block__init(dst, hd);
-    size_t field_count = certicoq_block__get_field_count(hd);
+    size_t field_count = certicoq_block__field_count_get(hd);
     size_t i;
     for (i = 0; i < field_count; i++)
     {
-        int_or_ptr f = certicoq_block__get_field(src, i);
-        certicoq_block__set_field(ret, i, f);
+        int_or_ptr f = certicoq_block__field_get(src, i);
+        certicoq_block__field_set(ret, i, f);
     }
     return ret;
 }
 
-certicoq_block_header_t *certicoq_block__get_header_ptr(const certicoq_block_t block)
+certicoq_block_header_t *certicoq_block__header_get_ptr(const certicoq_block_t block)
 {
     return (certicoq_block_header_t *)&block[-1];
 }
 
-void certicoq_block__set_header(certicoq_block_t block, const certicoq_block_header_t *header)
+void certicoq_block__header_set(certicoq_block_t block, const certicoq_block_header_t *header)
 {
     block[-1] = int_or_ptr__of_int(*header);
 }
 
-size_t certicoq_block__get_size(const certicoq_block_header_t *header)
+size_t certicoq_block__size_get(const certicoq_block_header_t *header)
 {
     const size_t zero = 0;
     const size_t one = 1;
     const size_t two = 2;
-    const size_t fc = certicoq_block__get_field_count(header);
+    const size_t fc = certicoq_block__field_count_get(header);
     return fc > zero ? one + fc : two;
 }
 
-size_t certicoq_block__get_field_count(const certicoq_block_header_t *header)
+size_t certicoq_block__field_count_get(const certicoq_block_header_t *header)
 {
-    return (header[0]) >> 10;
+    return header[0] >> 10;
 }
 
-void certicoq_block__set_field_count(certicoq_block_header_t *header, size_t size)
+void certicoq_block__field_count_set(certicoq_block_header_t *header, size_t size)
 {
-    header[0] = ((header[0]) & ~((1 << 10) - 1)) | (size << 10);
+    header[0] = (header[0] & ~((1 << 10) - 1)) | (size << 10);
 }
 
-certicoq_block_tag_t certicoq_block__get_tag(const certicoq_block_header_t *header)
+certicoq_block_tag_t certicoq_block__tag_get(const certicoq_block_header_t *header)
 {
-    return (header[0]) & 0xff;
+    return header[0] & 0xff;
 }
 
-certicoq_block_header_t certicoq_block__set_tag(certicoq_block_header_t *header, certicoq_block_tag_t tag)
+void certicoq_block__tag_set(certicoq_block_header_t *header, certicoq_block_tag_t tag)
 {
-    return ((header[0]) & ~0xff) | tag;
+    header[0] = (header[0] & ~0xff) | tag;
 }
 
-uint8_t certicoq_block__get_odata(const certicoq_block_header_t *header)
+uint8_t certicoq_block__odata_get(const certicoq_block_header_t *header)
 {
     return (header[0] >> 8) & 0x03;
 }
 
-void certicoq_block__set_odata(certicoq_block_header_t *header, uint8_t odata)
+void certicoq_block__odata_set(certicoq_block_header_t *header, uint8_t odata)
 {
     header[0] = (header[0] & ~(0x03 << 8)) | (odata << 8);
 }
 
-int_or_ptr *certicoq_block__get_field_ptr(certicoq_block_t block, size_t field)
+int_or_ptr *certicoq_block__field_get_ptr(certicoq_block_t block, size_t field)
 {
     return &block[field];
 }
 
-int_or_ptr certicoq_block__get_field(const certicoq_block_t block, size_t field)
+int_or_ptr certicoq_block__field_get(const certicoq_block_t block, size_t field)
 {
     return block[field];
 }
 
-void certicoq_block__set_field(certicoq_block_t block, size_t field, int_or_ptr x)
+void certicoq_block__field_set(certicoq_block_t block, size_t field, int_or_ptr x)
 {
     block[field] = x;
 }
