theories/Block/vst/verif/certicoq_block__odata_set.v
@@ -1,0 +1,21 @@
+From VST Require Import floyd.proofauto.
+
+From CertiCoq Require Import Block.vst.ast.ast.
+From CertiCoq Require Import Block.vst.clightgen.block.
+From CertiCoq Require Import Block.vst.cmodel.certicoq_block_header.
+From CertiCoq Require Import Block.vst.cmodel.certicoq_block.
+From CertiCoq Require Import Block.vst.spec.spec.
+
+Lemma body: semax_body Vprog ASI f_certicoq_block__odata_set certicoq_block__odata_set_spec.
+Proof.
+  start_function.
+  forward.
+  forward.
+  entailer!.
+  clear.
+  cbv [upd_Znth].
+  cbv [sublist].
+  unfold block_header_odata_set, block_header_encode_val.
+  simpl.
+  admit.
+Admitted.
